Add atomic and non-atomic variants of allocation

src/lang/memory.v
@@ -62,28 +62,6 @@ Notation store_view tv := (tv.1).1.
 Notation flush_view tv := (tv.1).2.
 Notation wb_buffer_view tv := (tv.2).
 
-(* Definition store_view (TV : thread_view) := (TV.1).1. *)
-(* Arguments store_view !TV. *)
-
-(* Definition flush_view (TV : thread_view) := (TV.1).2. *)
-(* Arguments flush_view TV /. *)
-
-(* Definition wb_buffer_view (TV : thread_view) : view := (TV.2). *)
-(* Arguments wb_buffer_view TV /. *)
-
-(* Lemma test (SV PV BV : view) : store_view (SV, PV, BV) = SV. *)
-(* Proof. simpl. reflexivity. Qed. *)
-
-(* Lemma test2 TV : store_view TV = (TV.1).1 ∧ app [1] [2] = [1; 2]. *)
-(* Proof. simpl. reflexivity. Qed. *)
-
-(* Global Instance store_view_mono : Proper ((⊑) ==> (⊑)) store_view. *)
-(* Proof. solve_proper. Qed. *)
-(* Global Instance flush_view_mono : Proper ((⊑) ==> (⊑)) flush_view. *)
-(* Proof. solve_proper. Qed. *)
-(* Global Instance wb_buffer_view_mono : Proper ((⊑) ==> (⊑)) wb_buffer_view. *)
-(* Proof. solve_proper. Qed. *)
-
 Notation history := (gmap time message).
 
 Notation store := (gmap loc history).
@@ -95,7 +73,7 @@ Section memory.
   Implicit Types (v : val) (ℓ : loc) (σ : store) (p : view).
 
   Inductive mem_event : Type :=
-  | MEvAllocN ℓ (len : nat) v
+  | MEvAllocN (a : memory_access) ℓ (len : nat) v
   | MEvLoad ℓ v
   | MEvStore ℓ v
   (* Acquire/release weak memory events. *)
@@ -110,21 +88,23 @@ Section memory.
   | MEvFenceSync.
 
   (* Takes a value and creates an initial history for that value. *)
-  Definition initial_history P v : history := {[0 := Msg v ∅ ∅ P]}.
+  Definition initial_history (a : memory_access) SV PV v : history :=
+    let view_access V := match a with NA => ∅ | AT => V end
+    in {[0 := Msg v (view_access SV) (view_access PV) PV]}.
 
   (* Convert an array into a store. *)
-  Fixpoint heap_array (l : loc) P (vs : list val) : store :=
+  Fixpoint heap_array ℓ a SV PV (vs : list val) : store :=
     match vs with
     | [] => ∅
-    | v :: vs' => {[ l := initial_history P v ]} ∪ heap_array (l +ₗ 1) P vs'
+    | v :: vs' =>
+        {[ ℓ := initial_history a SV PV v ]} ∪ heap_array (ℓ +ₗ 1) a SV PV vs'
     end.
 
-  Lemma heap_array_lookup (l : loc) P (vs : list val) (ow : history) (k : loc) :
-    (heap_array l P vs : store) !! k = Some ow ↔
-    (* True ↔ *)
-    ∃ j w, (0 ≤ j)%Z ∧ k = l +ₗ j ∧ (ow = {[0 := Msg w ∅ ∅ P]}) ∧ vs !! (Z.to_nat j) = (Some w).
+  Lemma heap_array_lookup ℓ a SV PV (vs : list val) (ow : history) (k : loc) :
+    (heap_array ℓ a SV PV vs : store) !! k = Some ow ↔
+    ∃ j w, (0 ≤ j)%Z ∧ k = ℓ +ₗ j ∧ (ow = initial_history a SV PV w) ∧ vs !! (Z.to_nat j) = (Some w).
   Proof.
-    revert k l; induction vs as [|v' vs IH]=> l' l /=.
+    revert k ℓ; induction vs as [|v' vs IH]=> l' ℓ /=.
     { rewrite lookup_empty. naive_solver lia. }
     rewrite -insert_union_singleton_l lookup_insert_Some IH. split.
     - intros [[-> ?] | (Hl & j & w & ? & -> & -> & ?)].
@@ -133,7 +113,7 @@ Section memory.
     - intros (j & w & ? & -> & -> & Hil). destruct (decide (j = 0)); simplify_eq/=.
       { rewrite loc_add_0; eauto. }
       right. split.
-      { rewrite -{1}(loc_add_0 l). intros ?%(inj (loc_add _)); lia. }
+      { rewrite -{1}(loc_add_0 ℓ). intros ?%(inj (loc_add _)); lia. }
       assert (Z.to_nat j = S (Z.to_nat (j - 1))) as Hj.
       { rewrite -Z2Nat.inj_succ; last lia. f_equal; lia. }
       rewrite Hj /= in Hil.
@@ -141,9 +121,9 @@ Section memory.
       auto with lia.
   Qed.
 
-  Lemma heap_array_map_disjoint (h : gmap loc history) P (l : loc) (vs : list val) :
-    (∀ i, (0 ≤ i)%Z → (i < length vs)%Z → h !! (l +ₗ i) = None) →
-    (heap_array l P vs) ##ₘ h.
+  Lemma heap_array_map_disjoint (h : gmap loc history) SV PV PAV ℓ (vs : list val) :
+    (∀ i, (0 ≤ i)%Z → (i < length vs)%Z → h !! (ℓ +ₗ i) = None) →
+    (heap_array ℓ SV PV PAV vs) ##ₘ h.
   Proof.
     intros Hdisj. apply map_disjoint_spec=> l' v1 v2.
     intros (j&w&?&->&?&Hj%lookup_lt_Some%inj_lt)%heap_array_lookup.
@@ -151,94 +131,93 @@ Section memory.
   Qed.
 
   (* Initializes a region of the memory starting at [ℓ] *)
-  Definition state_init_heap (ℓ : loc) (n : nat) P (v : val) (σ : store) : store :=
-    heap_array ℓ P (replicate n v) ∪ σ.
+  Definition state_init_heap a (ℓ : loc) (n : nat) SV PV (v : val) (σ : store) : store :=
+    heap_array ℓ a SV PV (replicate n v) ∪ σ.
 
   (* Small-step reduction steps on the memory. *)
 
   Inductive mem_step : mem_config → thread_view → mem_event → mem_config → thread_view → Prop :=
   (* Allocating a new location. *)
-  | MStepAllocN σ SV P B ℓ (len : nat) v p :
-     (0 < len)%Z → (* (∀ i, (0 ≤ i)%Z → (i < n)%Z → σ.(heap) !! (l +ₗ i) = None) → *)
+  | MStepAllocN a σ SV PV BV ℓ (len : nat) v p :
+     (0 < len)%Z → (* (∀ i, (0 ≤ i)%Z → (i < n)%Z → σ.(heap) !! (ℓ +ₗ i) = None) → *)
      (∀ idx, (0 ≤ idx)%Z → (idx < len)%Z → σ !! (ℓ +ₗ idx) = None) → (* This is a fresh segment of the heap not already in use. *)
      (* V' = <[ ℓ := 0 ]>SV → (* V' incorporates the new event in the threads view. *) This may not be needed. *)
-     mem_step (σ, p) (SV, P, B)
-              (MEvAllocN ℓ len v)
-              (state_init_heap ℓ len P v σ, p) (SV, P, B)
-              (* (<[ℓ := {[ 0 := Msg v V' P ]}]>σ, p) (V', P, B) *)
+     mem_step (σ, p) (SV, PV, BV)
+              (MEvAllocN a ℓ len v)
+              (state_init_heap a ℓ len SV PV v σ, p) (SV, PV, BV)
   (* A normal non-atomic load. *)
-  | MStepLoad (σ : store) SV P B t (ℓ : loc) (v : val) h p :
+  | MStepLoad (σ : store) SV PV BV t (ℓ : loc) (v : val) h p :
      σ !! ℓ = Some h →
      msg_val <$> (h !! t) = Some v →
-     ((SV !!0 ℓ)) ≤ t →
-     mem_step (σ, p) (SV, P, B)
+     (SV !!0 ℓ) ≤ t →
+     mem_step (σ, p) (SV, PV, BV)
               (MEvLoad ℓ v)
-              (σ, p) (SV, P, B)
-              (* (σ, p) ((<[ ℓ := t ]>SV), P, B) (* This variant includes the timestamp of the loaded msg. *) *)
+              (σ, p) (SV, PV, BV)
+              (* (σ, p) ((<[ ℓ := t ]>SV), PV, BV) (* This variant includes the timestamp of the loaded msg. *) *)
   (* An atomic acquire load. *)
-  | MStepLoadAcquire σ SV P B t ℓ (v : val) MV MP _MP h p :
+  | MStepLoadAcquire σ SV PV BV t ℓ (v : val) MV MP _MP h p :
      σ !! ℓ = Some h →
      (h !! t) = Some (Msg v MV MP _MP) →
      (SV !!0 ℓ) ≤ t →
-     mem_step (σ, p) (SV, P, B)
+     mem_step (σ, p) (SV, PV, BV)
               (MEvLoadAcquire ℓ v)
-              (σ, p) (SV ⊔ MV, P, B ⊔ MP) (* An acquire incorporates both the store view and the persistent view. *)
+              (σ, p) (SV ⊔ MV, PV, BV ⊔ MP) (* An acquire incorporates both the store view and the persistent view. *)
   (* A normal non-atomic write. *)
-  | MStepStore σ SV P B t ℓ (v : val) h V' p :
+  | MStepStore σ SV PV BV t ℓ (v : val) h V' p :
      σ !! ℓ = Some h →
      (h !! t) = None → (* No event exists at t already. *)
      (SV !!0 ℓ) < t →
      V' = <[ℓ := MaxNat t]>SV → (* V' incorporates the new event in the threads view. *)
-     mem_step (σ, p) (SV, P, B)
+     mem_step (σ, p) (SV, PV, BV)
              (MEvStore ℓ v)
-             (<[ℓ := <[t := Msg v ∅ ∅ P]>h]>σ, p) (V', P, B)
+             (<[ℓ := <[t := Msg v ∅ ∅ PV]>h]>σ, p) (V', PV, BV)
   (* An atomic release write. *)
-  | MStepStoreRelease σ SV P B t ℓ (v : val) h V' p :
+  | MStepStoreRelease σ SV PV BV t ℓ (v : val) h V' p :
      σ !! ℓ = Some h →
      (h !! t) = None → (* No event exists at t already. *)
      (SV !!0 ℓ) < t →
      V' = <[ℓ := MaxNat t]>SV → (* V' incorporates the new event in the threads view. *)
-     mem_step (σ, p) (SV, P, B)
+     mem_step (σ, p) (SV, PV, BV)
               (MEvStoreRelease ℓ v)
-              (<[ℓ := <[t := Msg v V' P P]>h]>σ, p) (V', P, B) (* A release releases both V' and P. *)
+              (<[ℓ := <[t := Msg v V' PV PV]>h]>σ, p) (V', PV, BV) (* A release releases both V' and PV. *)
   (* Read-modify-write instructions. *)
-  | MStepRMW σ ℓ h v MV MP S t S' P P' B p v' _MP :
+  | MStepRMW σ ℓ h v MV MP SV t S' PV P' BV p v' _MP :
      σ !! ℓ = Some h →
-     (S !!0 ℓ) ≤ t →
+     (SV !!0 ℓ) ≤ t →
      (h !! t) = Some (Msg v MV MP _MP) → (* We read an event at time [t]. *)
      (* All values that we could have reads are comparable to [v]. *)
-     (∀ t' msg, S !!0 ℓ ≤ t' → h !! t' = Some msg → vals_compare_safe msg.(msg_val) v) →
+     (∀ t' msg, SV !!0 ℓ ≤ t' → h !! t' = Some msg → vals_compare_safe msg.(msg_val) v) →
      (h !! (t + 1)) = None → (* The next timestamp is available, ensures that no other RMW read this event. *)
-     S' = (<[ ℓ := MaxNat (t + 1) ]>(S ⊔ MV)) → (* S' incorporates the new event in the threads view. *)
-     P' = P ⊔ MP →
-     mem_step (σ, p) (S, P, B)
+     S' = (<[ ℓ := MaxNat (t + 1) ]>(SV ⊔ MV)) → (* S' incorporates the new event in the threads view. *)
+     P' = PV ⊔ MP →
+     mem_step (σ, p) (SV, PV, BV)
               (MEvRMW ℓ v v')
-              (<[ℓ := <[t := Msg v S' P' P']>h]>σ, p) (S', P, B ⊔ MP)
-  | MStepRMWFail σ S P B t ℓ (v : val) MV MP _MP h p :
+              (<[ℓ := <[t := Msg v S' P' P']>h]>σ, p) (S', PV, BV ⊔ MP)
+  | MStepRMWFail σ SV PV BV t ℓ (v : val) MV MP _MP h p :
      σ !! ℓ = Some h →
      (h !! t) = Some (Msg v MV MP _MP) →
-     (S !!0 ℓ) ≤ t →
-     (∀ t' msg, S !!0 ℓ ≤ t' → h !! t' = Some msg → vals_compare_safe msg.(msg_val) v) →
-     mem_step (σ, p) (S, P, B)
+     (SV !!0 ℓ) ≤ t →
+     (∀ t' msg, SV !!0 ℓ ≤ t' → h !! t' = Some msg → vals_compare_safe msg.(msg_val) v) →
+     mem_step (σ, p) (SV, PV, BV)
               (MEvLoadEx ℓ v)
-              (σ, p) (S ⊔ MV, P, B ⊔ MP) (* An acquire incorporates both the store view and the persistent view. *)
+              (σ, p) (SV ⊔ MV, PV, BV ⊔ MP) (* An acquire incorporates both the store view and the persistent view. *)
   (* Write-back instruction. *)
-  | MStepWB σ SV P B ℓ t p :
+  | MStepWB σ SV PV BV ℓ t p :
      (* σ !! ℓ = Some h → *)
      (SV !!0 ℓ) = t → (* An equality here is fine, the timestamps are only lower bounds anyway. *)
-     mem_step (σ, p) (SV, P, B)
+     mem_step (σ, p) (SV, PV, BV)
               (MEvWB ℓ)
-              (σ, p) (SV, P, {[ℓ := MaxNat t]} ⊔ B)
+              (σ, p) (SV, PV, {[ℓ := MaxNat t]} ⊔ BV)
   (* Asynchronous fence. *)
-  | MStepFence σ SV P B p :
-     mem_step (σ, p) (SV, P, B)
+  | MStepFence σ SV PV BV p :
+     mem_step (σ, p) (SV, PV, BV)
               MEvFence
-              (σ, p) (SV, P ⊔ B, B)
+              (σ, p) (SV, PV ⊔ BV, BV)
   (* Synchronous fence. *)
-  | MStepFenceSync σ SV P B p :
-     mem_step (σ, p) (SV, P, B)
+  | MStepFenceSync σ SV PV BV p :
+     mem_step (σ, p) (SV, PV, BV)
               MEvFenceSync
-              (σ, p ⊔ B) (SV, P ⊔ B, B).
+              (σ, p ⊔ BV) (SV, PV ⊔ BV, BV).
 
   (* Removes all messages from [hist] after [t]. *)
   Definition cut_history t (hist : history) : history :=
@@ -270,12 +249,12 @@ Section memory.
      crash_step (σ, p) (slice_of_store p' σ, view_to_zero p').
 
   (* It is always possible to allocate a section of memory. *)
-  Lemma alloc_fresh v (len : nat) σ p SV P B :
+  Lemma alloc_fresh v (len : nat) a σ p SV PV BV :
     let ℓ := fresh_locs (dom (gset loc) σ) in (* ℓ is directly after the largest allocated location. *)
     (0 < len)%Z →
-    mem_step (σ, p) (SV, P, B)
-             (MEvAllocN ℓ len v)
-             (state_init_heap ℓ len P v σ, p) (SV, P, B).
+    mem_step (σ, p) (SV, PV, BV)
+             (MEvAllocN a ℓ len v)
+             (state_init_heap a ℓ len SV PV v σ, p) (SV, PV, BV).
   Proof.
     intros. apply MStepAllocN; first done.
     intros. apply not_elem_of_dom.
